interpreting LatticeAlg into functional Lattice

examples/layeredeffects/LatticeAlg.fst
@@ -8,7 +8,6 @@ open FStar.Universe
 
 module WF = FStar.WellFounded
 
-
 #set-options "--print_universes --print_implicits --print_effect_args"
 
 // GM: Force a type equality by SMT
@@ -113,33 +112,30 @@ let rec sublist_at
     | [] -> ()
     | _::l1 -> sublist_at l1 l2
 
-let rec abides_sublist #a (l1 l2 : list eff_label) (c : repr0 a)
+let rec abides_sublist_nopat #a (l1 l2 : list eff_label) (c : repr0 a)
   : Lemma (requires (abides (interp l1) c) /\ sublist l1 l2)
           (ensures (abides (interp l2) c))
-          [SMTPat (abides (interp l2) c); SMTPat (sublist l1 l2)]
   = match c with
     | Return _ -> ()
     | Act a i k -> 
       let sub o : Lemma (abides (interp l2) (k o)) =
         FStar.WellFounded.axiom1 k o;
-        abides_sublist l1 l2 (k o)
+        abides_sublist_nopat l1 l2 (k o)
       in
       Classical.forall_intro sub
+      
+let abides_sublist #a (l1 l2 : list eff_label) (c : repr0 a)
+  : Lemma (requires (abides (interp l1) c) /\ sublist l1 l2)
+          (ensures (abides (interp l2) c))
+          [SMTPat (abides (interp l2) c); SMTPat (sublist l1 l2)]
+  = abides_sublist_nopat l1 l2 c
 
-let rec abides_app #a (l1 l2 : list eff_label) (c : repr0 a)
+let abides_app #a (l1 l2 : list eff_label) (c : repr0 a)
   : Lemma (requires (abides (interp l1) c \/ abides (interp l2) c))
           (ensures (abides (interp (l1@l2)) c))
           [SMTPat (abides (interp (l1@l2)) c)]
-  = // GM: Just copied the proof from above since it ought to work,
-    //     do something smarter later.
-    match c with
-    | Return _ -> ()
-    | Act a i k -> 
-      let sub o : Lemma (abides (interp (l1@l2)) (k o)) =
-        FStar.WellFounded.axiom1 k o;
-        abides_app l1 l2 (k o)
-      in
-      Classical.forall_intro sub
+  = Classical.move_requires (abides_sublist_nopat l1 (l1@l2)) c;
+    Classical.move_requires (abides_sublist_nopat l2 (l1@l2)) c
 
 let return (a:Type) (x:a)
   : repr a []
@@ -298,9 +294,6 @@ let catchST #a #labs
    _catchST (reify (f ())) s0
  end
 
-// TODO: haskell-like runST.
-// strong update with index on state type(s)?
-
 let g #labs () : EFF int labs = 42  //AR: 07/03: had to hoist after removing smt_reifiablep
 
 let test_catch #labs (f : unit -> EFF int [EXN;WR]) : EFF int [WR] =
@@ -385,6 +378,9 @@ let handler_ty_l (l:eff_label) (b:Type) (labs:list eff_label) =
   //let (| _, _, a |) = action_of l in
   //handler_ty a b labs
 
+(* A generic handler for a (single) label l, relies on the fact that
+we can compare actions for equality, or equivalently map them to their
+labels. *)
 val handle (#a:_) (#labs:_) (l:eff_label)
            (f:repr a (l::labs))
            (h:handler_ty_l l a labs)
@@ -402,62 +398,60 @@ let rec handle #a #labs l f h =
       in
       Act act i k'
     end
-    
+
 let catch0' #a #labs (t1 : repr a (EXN::labs))
-                         (t2 : repr a labs)
+                      (t2 : repr a labs)
   : repr a labs
   = handle EXN t1 (fun i k -> t2)
   
-open Lattice
+module L = Lattice
 
 let trlab = function
-  | RD  -> Lattice.RD
-  | WR  -> Lattice.WR
-  | EXN -> Lattice.EXN
+  | RD  -> L.RD
+  | WR  -> L.WR
+  | EXN -> L.EXN
+  
+let trlab' = function
+  | L.RD  -> RD
+  | L.WR  -> WR
+  | L.EXN -> EXN
 
-let trlabs = List.Tot.map trlab
+let trlabs  = List.Tot.map trlab
+let trlabs' = List.Tot.map trlab'
 
-[@@expect_failure] // todo this should work
+let rec lab_corr (l:eff_label) (ls:list eff_label)
+  : Lemma (mem l ls <==> mem (trlab l) (trlabs ls))
+          [SMTPat (mem l ls)] // needed for interp_into_lattice_repr below
+  = match ls with
+    | [] -> ()
+    | l1::ls -> lab_corr l ls
+
+(* Tied to the particular repr of Lattice.fst *)
+
 let rec interp_into_lattice_repr #a #labs
   (t : repr a labs)
-  : Lattice.repr a (trlabs labs)
+  : L.repr a (trlabs labs)
   = match t with
-    | Return x -> Lattice.return _ x
-    | Act Read _ k -> (fun s0 -> WF.axiom1 k s0; interp_into_lattice_repr #a #labs (k s0) s0)
-    | Act Write s k -> (fun s0 -> WF.axiom1 k (); interp_into_lattice_repr #a #labs (k ()) s)
-    | Act Raise e k -> (fun s0 -> (None, s0))
+    | Return x -> L.return _ x
+    | Act Read i k -> 
+      L.bind _ _ _ _ (reify (L.get i))
+       (fun x -> WF.axiom1 k x;
+              interp_into_lattice_repr #a #labs (k x))
+    | Act Write i k -> 
+      L.bind _ _ _ _ (reify (L.put i))
+       (fun x -> WF.axiom1 k x;
+              interp_into_lattice_repr #a #labs (k x))
+    | Act Raise i k -> 
+      L.bind _ _ _ _ (reify (L.raise ()))
+       (fun x -> WF.axiom1 k x;
+              interp_into_lattice_repr #a #labs (k x))
 
-//let interp_into_lattice #a #labs
-//  (f : unit -> EFF a labs)
-//  : Lattice.EFF a (trlabs labs)
-//  = Lattice.EFF?.reflect (interp_into_lattice_repr (reify (f ())))
-//
-//let interp_full #a #labs
-//  (f : unit -> EFF a labs)
-//  : Tot (f:(state -> Tot (option a & state)){Lattice.abides f (Lattice.interp (trlabs labs))})
-//  = reify (interp_into_lattice #a #labs f)
+let interp_into_lattice #a #labs
+  (f : unit -> EFF a labs)
+  : Lattice.EFF a (trlabs labs)
+  = Lattice.EFF?.reflect (interp_into_lattice_repr (reify (f ())))
 
-
-type sem0 (a:Type u#aa) : Type u#aa =
-  state -> Tot (option a & state)
-
-let abides' #a (f : sem0 a) (ann:annot) : prop =
-    (ann RD  = false ==> (forall s0 s1. fst (f s0) == fst (f s1)))
-  /\ (ann WR  = false ==> (forall s0. snd (f s0) == s0))
-  /\ (ann EXN = false ==> (forall s0. Some? (fst (f s0))))
-
-type sem (a:Type u#aa) (labs : list u#0 eff_label) // #2074 : Type u#aa
-  =
-  r:(sem0 a){abides' r (interp labs)}
-
-//let rec interp_sem #a #labs (t : repr a labs) : sem a labs =
-//  let r (s0:state) : Tot (option a & state) =
-//    match t with
-//    | Return x -> (Some x, s0)
-//    | Act Read _ k -> WF.axiom1 k s0; interp_sem #a #labs (k s0) s0
-//    | Act Write s k -> WF.axiom1 k (); interp_sem #a #labs (k ()) s
-//    | Act Raise e k -> (None, s0)
-//  in
-//  assume (not (mem RD labs));
-//  assume (mem EXN labs);
-//  r
+let interp_full #a #labs
+  (f : unit -> EFF a labs)
+  : Tot (f:(state -> Tot (option a & state)){Lattice.abides f (Lattice.interp (trlabs labs))})
+  = reify (interp_into_lattice #a #labs f)
